@prefix cpe: <http://cpe.mitre.org/dictionary/2.0> .
@prefix rdf: <http://www.w3.org/1999/02/22-rdf-syntax-ns#> .
@prefix rdfs: <http://www.w3.org/2000/01/rdf-schema#> .

##
## Generator Type
##

cpe:GeneratorType rdf:type rdfs:Class ;
    rdfs:comment "The Generator defines an element that is used to hold information about when a particular document was compiled" ;
    rdfs:label "Generator" ;
    .
    
cpe:product_name rdf:type rdf:Property ;
    rdfs:comment "The optional product_name element specifies the name of the application used to generate the file." ; 
    rdfs:domain cpe:GeneratorType ;
    rdfs:range rdfs:Literal ;
    rdfs:label "Product Name" ;
    .
    
cpe:product_version rdf:type rdf:Property ;
    rdfs:comment "The optional product_version element specifies the version of the application used to generate the file." ; 
    rdfs:domain cpe:GeneratorType ;
    rdfs:range rdfs:Literal ;
    rdfs:label "Product Version" ;
    .
    
cpe:schema_version rdf:type rdf:Property ;
    rdfs:comment "The required schema_version element specifies the version of the schema that the document has been written against and that should be used for validation." ; 
    rdfs:domain cpe:GeneratorType ;
    rdfs:range rdfs:Literal ;
    rdfs:label "Schema Version" ;
    .
    
cpe:timestamp rdf:type rdf:Property ;
    rdfs:comment """The required timestamp element specifies when the particular
                        document was compiled. The format for the timestamp is yyyy-mm-ddThh:mm:ss. Note that the
                        timestamp element does not specify when an item in the document was created or modified but
                        rather when the actual XML document that contains the items was created. For example, a document
                        might pull a bunch of existing items together, each of which was created at some point in the
                        past. The timestamp in this case would be when this combined document was
                        created.""" ;
    rdfs:domain cpe:GeneratorType ;
    rdfs:range rdfs:Literal ;
    rdfs:label "Creaton Date" ;
    .    
  
##
## Item Type
##  
    
cpe:ItemType rdf:type rdf:Class ;
    rdfs:comment "The ItemType defines a class that represents a single CPE Name and should follow the URI structure outlined in the CPE Specification." ;
    rdfs:label "ItemType" .

cpe:cpe-item rdf:type rdf:Property ;
    rdfs:comment "The cpe-item property points to an ItemType" ;
    rdfs:domain rdfs:Resource ;
    rdfs:range cpe:ItemType ;
    rdfs:label "CPE item" ;
    .

cpe:title rdf:type rdf:Property ;
    rdfs:comment "The optional title property is used to provide a human-readable title for the platform." ;
    rdfs:domain cpe:ItemType ;
    rdfs:range rdfs:Literal ;
    rdfs:label "Title" ;
    .

cpe:deprecated rdf:type rdf:Property ;
    rdfs:comment "A flag that indicates the CPE is deprecated" ;
    rdfs:domain cpe:ItemType ;
    rdfs:range rdfs:Literal ;
    rdfs:label "Deprecated" ;
    .

cpe:note rdf:type rdf:Property ;
    rdfs:comment "The optional notes property is used to provide a human-readable descriptive material." ;
    rdfs:domain cpe:ItemType ;
    rdfs:range rdfs:Literal ;
    rdfs:label "Note" ;
    .

cpe:reference rdf:type rdf:Property ;
    rdfs:comment "The optional reference property contains links to external resources." ;
    rdfs:domain cpe:ItemType ;
    rdfs:range cpe:ReferenceType ;
    rdfs:label "References" ;
    .

cpe:check rdf:type rdf:Property ;
    rdfs:comment "The optional check element is used to call out an OVAL Definition URL that can confirm or reject an IT system as an instance of the named platform." ;
    rdfs:domain cpe:ItemType ;
    rdfs:range cpe:CheckType ;
    rdfs:label "Check" ;
    .
    
cpe:name rdf:type rdf:Property ;
    rdfs:comment "a single CPE Name" ;
    rdfs:range rdfs:Literal ;
    rdfs:label "Name" ;
    .

cpe:deprecated_by rdf:type rdf:Property ;
    rdfs:comment "The Item that deprecated this item" ;
    rdfs:domain cpe:ItemType ;
    rdfs:range cpe:ItemType ;
    rdfs:label "Deprecated by" ;
    .

cpe:deprecation_date rdf:type rdf:Property ;
    rdfs:comment "The data this item was deprecated" ;
    rdfs:domain cpe:ItemType ;
    rdfs:range rdfs:Literal ;
    rdfs:label "Deprecation date" ;
    .

##
## Reference Type
##

cpe:ReferenceType rdf:type rdf:Class ;
    rdfs:comment "The ReferenceType defines a class that contains references." ;
    rdfs:label "ReferenceType" ;
    .
    
cpe:reference rdf:type rdf:Property ;
    rdfs:comment "The optional reference property contains links to external resources." ;
    rdfs:domain cpe:ReferenceType ;
    rdfs:range rdfs:Literal ;
    rdfs:label "Reference Type" ;
    .
    
##
## Check Type
##

cpe:CheckType rdf:type rdf:Class ;
    rdfs:comment "The ReferenceType defines a class that contains references." ;
    rdfs:label "CheckType" ;
    .

cpe:system rdf:type rdf:Property ;
    rdfs:comment "The URI for a particular version of OVAL or a related system testing language." ;
    rdfs:domain cpe:CheckType ;
    rdfs:range rdfs:Resource ;
    rdfs:label "Testing System" ;
    .

cpe:href rdf:type rdf:Property ;
    rdfs:comment "An external file reference." ;
    rdfs:domain cpe:ReferenceType ;
    rdfs:range rdfs:Resource ;
    rdfs:label "Content Test Identifier" ;
    
    
    .
    
   
