@prefix cpe23: <http://scap.nist.gov/schema/cpe-extension/2.3> .
@prefix cpe: <http://cpe.mitre.org/dictionary/2.0> .
@prefix rdf: <http://www.w3.org/1999/02/22-rdf-syntax-ns#> .
@prefix rdfs: <http://www.w3.org/2000/01/rdf-schema#> .


##
## Item Type
##

cpe23:ItemType rdf:type rdfs:Class ;
    rdfs:comment """This class captures all CPE 2.3 specific data including the CPE 2.3
                formatted string binding of the name, provenance data, and deprecation data. """ ;
    rdfs:label "CPE 2.3 Item Type" ;
    .
    
cpe23:cpe23-item rdf:type rdf:Property ;
    rdfs:comment "a pointer to an CPE 2.3 item." ; 
    rdfs:range cpe23:Resource ;
    rdfs:range cpe23:ItemType ;
    rdfs:label "CPE 2.3 Item" ;
    .
        
cpe23:provenance-record rdf:type rdf:Property ;
    rdfs:comment "a pointer to the provenance data." ; 
    rdfs:domain cpe23:ItemType ;
    rdfs:range cpe23:provenanceRecordType ;
    rdfs:label "Provenance" ;
    .
    
cpe23:deprecation rdf:type rdf:Property ;
    rdfs:comment "A pointer to a deprecation entrie for the given identifier name." ; 
    rdfs:domain cpe23:ItemType ;
    rdfs:range cpe23:deprecationType ;
    rdfs:label "Deprecation" ;    
    .
    
cpe23:name rdf:type rdf:Property ;
    rdfs:comment "the CPE 2.3 item name." ; 
    rdfs:range rdfs:Literal ;
    rdfs:label "Name" ;    
    .
    
##
## Provenance record type
##

cpe23:provenanceRecordType rdf:type rdfs:Class ;
    rdfs:comment "Class holding all provenance information for the given identifier." ;
    rdfs:label "Provenance Type" ;
    .

cpe23:submitter rdf:type rdf:Property ;
    rdfs:comment "The organization responsible for submitting the identifier name." ; 
    rdfs:domain cpe23:provenanceRecordType ;
    rdfs:range cpe23:organizationType ;
    rdfs:label "Submitter" ;
    .
    
cpe23:authority rdf:type rdf:Property ;
    rdfs:comment "The authority responsible for endorsing the identifier name. Multiple authorities may endorse the same identifier name." ; 
    rdfs:domain cpe23:provenanceRecordType ;
    rdfs:range cpe23:organizationType ;
    rdfs:label "Authority" ;
    .

cpe23:change-description rdf:type rdf:Property ;
    rdfs:comment "A description of any changes made to the identifier name or associated metadata." ; 
    rdfs:domain cpe23:provenanceRecordType ;
    rdfs:range cpe23:changeDescriptionType ;
    rdfs:label "Authority" ;
    .
  
##
## Change description Type
##

cpe23:changeDescriptionType rdf:type rdfs:Class ;
    rdfs:comment "A description of any changes made to the identifier name or associated metadata." ; 
    rdfs:label "Change Description Type" ;
    .
    
cpe23:evidence-reference rdf:type rdf:Property ;
    rdfs:comment "Supporting evidence for any changes to a name or associated metadata, including a link to external information relating to the change." ; 
    rdfs:domain cpe23:provenanceRecordType ;
    rdfs:range cpe23:evidenceReferenceType ;
    rdfs:label "Evidence Reference" ;
    .
    
cpe23:comments rdf:type rdf:Property ;
    rdfs:comment "Comments explaining the rationale for the change." ; 
    rdfs:domain cpe23:provenanceRecordType ;
    rdfs:range rdfs:Literal ;
    rdfs:label "Comments" ;
    .    

cpe23:change-type rdf:type rdf:Property ;
    rdfs:comment "The type of change that occurred." ; 
    rdfs:domain cpe23:provenanceRecordType ;
    rdfs:range rdfs:Literal ;
    rdfs:label "Change Type" ;
    .    
        
cpe23:date rdf:type rdf:Property ;
    rdfs:comment "When the change occurred." ; 
    rdfs:range rdfs:Literal ;
    rdfs:label "Date of Change" ;
    .    
        
##
## Deprecation Type type
##

cpe23:deprecationType rdf:type rdfs:Class ;
    rdfs:comment """An element containing information for a specific deprecation of an
                identifier name. A single deprecation element may contain a list of names that the enclosing identifier
                name was deprecated by. One deprecation element represents a deprecation that occurred at a specific
                instant in time; it is possible that additional deprecations will occur at a later instant in time. If a
                dictionary maintainer must submit deprecation entries after the initial deprecation, then another
                deprecation element should be added to the identifier name. """ ;
    rdfs:label "Deprecation Type" ;
    .

cpe23:deprecated-by rdf:type rdf:Property ;
    rdfs:comment "the names that deprecated the identifier name. The names in the list do not have to be identifier names; they may contain wildcards and represent sets of products." ; 
    rdfs:domain cpe23:deprecationType ;
    rdfs:range rdfs:Literal ;
    rdfs:label "Deprecated by" ;
    .

##
##  deprecated info type
##    
cpe23:deprecatedInfoType rdf:type rdfs:Class ;
    rdfs:comment "The name that is deprecating the identifier name." ; 
    rdfs:label "Deprecation Type" ;
    .

cpe23:type rdf:type rdf:Property ;
    rdfs:comment "the type of deprecaton" ; 
    rdfs:domain cpe23:deprecationType ;
    rdfs:range rdfs:Literal ;
    rdfs:label "Deprecated by" ;
    .
    
##
## Organization type
##

cpe23:organizationType rdf:type rdfs:Class ;
    rdfs:comment "A description of an orgianization." ; 
    rdfs:label "Organization Type" ;
    .
    
cpe23:description rdf:type rdf:Property ;
    rdfs:comment "A high-level description of the organization acting as the submitter or authority. " ; 
    rdfs:domain cpe23:organizationType ;
    rdfs:range rdfs:Literal ;
    rdfs:label "Description" ;
    .
    
##
## Evidence Reference Type
##

cpe23:evidenceReferenceType rdf:type rdfs:Class ;
    rdfs:comment "Supporting evidence for any changes to a name or associated metadata, including a link to external information relating to the change." ; 
    rdfs:label "Evidence Reference Type" ;
    .
    
cpe23:evidenceType rdf:type rdf:Property ;
    rdfs:comment "The type of evidence" ; 
    rdfs:domain cpe23:evidenceReferenceType ;
    rdfs:range rdfs:Resource ;
    rdfs:label "Evidence Type" ;
    .
